ROOT
@@ -1,14 +1,5 @@
 chapter AFP
 
-session FO_proof_systems in "FO_proof_systems" = HOL +
-  description \<open>Something between propositional and first-order logic\<close>
-  sessions
-    "HOL-Library"
-  theories
-    Formulas
-    Sema
-    Consistency
-
 session AI_Planning_Languages_Semantics_With_Quantifiers = HOL +
   description \<open>AI Planning Languages Semantics and Validation\<close>
   options [timeout = 600]
@@ -17,6 +8,7 @@ session AI_Planning_Languages_Semantics_With_Quantifiers = HOL +
     "Certification_Monads"
     "Show"
     "Containers"
+    "Propositional_Proof_Systems"
   theories [document = false]
     "HOL-Library.Code_Target_Nat"
     "HOL-Library.Monad_Syntax"
